Vol3/exercise2.v
@@ -1,0 +1,125 @@
+Set Warnings "-notation-overridden,-parsing,-deprecated-hint-without-locality".
+From VFA Require Import exercise1.
+
+Fixpoint insert (n : nat) (l : list nat) : list nat :=
+  match l with
+  | [] => [n]
+  | n' :: l' => if n' >? n then n :: n' :: l' else n' :: (insert n l')
+  end.
+
+Fixpoint sort (l : list nat) : list nat :=
+  match l with
+  | [] => []
+  | n :: l' => insert n (sort l')
+  end.
+
+Inductive sorted : list nat -> Prop :=
+  | sorted_nil :
+      sorted []
+  | sorted_1 : forall x,
+      sorted [x]
+  | sorted_cons : forall x y l,
+      x <= y -> sorted (y :: l) -> sorted (x :: y :: l).
+
+Definition sorted' (l : list nat) := forall i j iv jv,
+  i < j ->
+  nth_error l i = Some iv ->
+  nth_error l j = Some jv ->
+  iv <= jv.
+
+Definition sorted'' (l : list nat) := forall i j,
+  i < j < length l ->
+  nth i l 0 <= nth j l 0.
+
+Definition is_a_sorting_algorithm (f: list nat -> list nat) := forall l,
+  Permutation l (f l) /\ sorted (f l).
+
+Lemma le_gt_false : forall x y,
+  x <= y -> x >? y = false.
+Proof.
+  intros. bdestruct (x >? y).
+  - lia.
+  - reflexivity.
+Qed.
+
+(* **** Exercise: 3 stars, standard (insert_sorted) *)
+(* Prove that insertion maintains sortedness. Make use of tactic
+    bdestruct, defined in Perm. *)
+Lemma sorted_is_sorted : forall x y,
+  x <= y -> sorted [x; y].
+Proof.
+  intros. apply sorted_cons. apply H. apply sorted_1.
+Qed.
+
+Lemma ge_false : forall x y,
+  x >= y -> ~ (y > x).
+Proof.
+  intros. lia.
+Qed.
+
+Lemma insert_sorted:
+  forall a l, sorted l -> sorted (insert a l).
+Proof.
+  intros. induction H.
+  - apply sorted_1.
+  - simpl. bdestruct (x >? a); apply sorted_is_sorted; lia.
+  - simpl. bdestruct (x >? a). apply sorted_cons. lia. apply sorted_cons. lia. apply H0.
+    bdestruct (y >? a). apply sorted_cons. lia. apply sorted_cons. lia. apply H0.
+    apply sorted_cons. apply H.
+    simpl in IHsorted.
+    bdestruct (y >? a).
+    * apply ge_false in H2. unfold not in H2. apply H2 in H3. inversion H3.
+    * apply IHsorted.
+Qed.
+
+(** **** Exercise: 2 stars, standard (sort_sorted) *)
+(* Using insert_sorted, prove that insertion sort makes a list sorted. *)
+Theorem sort_sorted: forall l, sorted (sort l).
+Proof.
+  intros. induction l.
+  - apply sorted_nil.
+  - simpl. apply insert_sorted. apply IHl.
+Qed.
+
+(** **** Exercise: 3 stars, standard (insert_perm) *)
+(* The following lemma will be useful soon as a helper. Take advantage of helpful theorems from the
+Permutation library. *)
+Lemma insert_perm: forall x l,
+    Permutation (x :: l) (insert x l).
+Proof.
+  intros. induction l.
+  - simpl. apply Permutation_refl.
+  - simpl. bdestruct (a >? x).
+    + apply Permutation_refl.
+    + apply perm_trans with (a :: x :: l).
+      * apply perm_swap.
+      * apply perm_skip. apply IHl.
+Qed.
+
+(** **** Exercise: 3 stars, standard (sort_perm) *)
+(* Prove that sort is a permutation, using insert_perm. *)
+Theorem sort_perm: forall l, Permutation l (sort l).
+Proof.
+  intros. induction l.
+  - apply perm_nil.
+  - simpl. apply perm_trans with (a :: sort l).
+    + apply perm_skip. apply IHl.
+    + apply insert_perm.
+Qed.
+
+(* Exercise: 1 star, standard (insertion_sort_correct) *)
+(* Finish the proof of correctness! *)
+Theorem insertion_sort_correct:
+    is_a_sorting_algorithm sort.
+Proof.
+  intros. split.
+  - apply sort_perm.
+  - apply sort_sorted.
+Qed.
+
+(* Summary: *)
+(* 
+  First, we need to define what a sorting algorithm is:
+    - It should be a permutation of the original list.
+    - It should be a 
+*)
